# Chapter 1 Exercises

## Intermission: Equivalence exercises

1. `λxy.xz`: B `λmn.mz`
2. `λxy.xxy`: C `λa.(λb.aab)`
3. `λxyz.zx`: B `λtos.st`

## Exercises

**Which are combinators?**

1. `λx.xxx` : Yes
2. `λxy.zx` : No
3. `λxyz.xy(zx)` : Yes
4. `λxyz.xy(zxy)` : Yes
5. `λxy.xy(zxy)` : No

**Normal form or diverge?**

1. λx.xxx : No

2. (λz.zz)(λy.yy)
   (λy.yy)(λy.yy) : Yes

3. (λx.xxx)z
   zzz : No

**Beta Reduction**

# 1. (λabc.cba)zz(λwv.w)

```haskell
(λabc.cba)zz(λwv.w)

(λbc.cbz)z(λwv.w)

(λc.czz)(λwv.w)

(λwv.w)zz

(λv.z)z

z

```

# 2. (λx.λy.xyy)(λa.a)b

```
(λx.λy.xyy)(λa.a)b

(λy.(λa.a)yy)b

(λa.a)bb

bb
```

# 3 (λy.y)(λx.xx)(λz.zq)

```
(λy.y)(λx.xx)(λz.zq)

(λx.xx)(λz.zq)

(λz.zq)(λz.zq)

(λz.zq)q

qq

```

# 4 (λz.z)(λz.zz)(λz.zy)

```
(λz.z)(λz.zz)(λz.zy)

(λz.zz)(λz.zy)

(λz.zy)(λz.zy)

(λz.zy)y

yy

```

# 5 (λx.λy.xyy)(λy.y)y

```
a. (λx.λy.xyy)(λy.y)y

b. (λy.(λy.y)yy)y | (𝜆𝑦.(𝜆𝑦.𝑦)𝑦𝑦)𝑦

c. (λy.yy)y | (𝜆𝑦.𝑦)𝑦𝑦

yy

```

I got the same answer but, in (c) I replaced the inner/second `λy` with the innder `yy`. The book replaces the outer/first `λy` with `y`. _Is my approach correct?_

# 6. (λa.aa)(λb.ba)c

```
(λa.aa)(λb.ba)c

(λb.ba)(λb.ba)c

(λb.ba)ac

aac

```

# 7. (λxyz.xz(yz))(λx.z)(λx.a)

Book Solution

```haskell
(λxyz.xz(yz))(λx.z)(λx.a) -- a
(λyz'.(λx.z)z'(yz))(λx.a) -- b

λz'.(λx.z)z' ((λx.a)z) -- c
λz'.z        ((λx.a)z) -- d

(d)
-- I apply z' to λx.z
-- remove the head and z goes away because when a λ is applied to a free & the body has a free variable, the head is removed and the free variable is tossed. All that remains is the term t which the λ is being applied.

-- When a λ with no bound variables is applied to a variable/term, the variable/term it is applied to goes away because it is not referenced in the body of the λ. What remains is the free variables.
-- Example (λx.z)a -> z
   -- a is tossed and the head is removed leave only z


λz'.za -- e
```

My try

```haskell
(λxyz.xz(yz))(λx.z)(λx.a)
(λxyz'.xz'(yz))(λx.z)(λx.a)
(λyz'.(λx.z)z'(yz))(λx.a)
(λz'.(λx.z)z'((λx.a)z))
(λz'.z((λx.a)z))
(λz'.za)


```

Try again

```haskell
(λxyz.xz(yz))(λx.z)(λx.a)
-- alpha replace first z with z'
(λxyz'.xz'(yz))(λx.z)(λx.a)
-- replace x with (λx.z)
(λyz'.(λx.z)z'(yz))(λx.a)
-- replace y with (λx.a)
(λz'.(λx.z)z'((λx.a)z))
-- replace the first λx with z'
(λz'.z((λx.a)z))
-- replace λx with z
(λz'.z((a)))
-- remove paren
λz'.za
```

OK, I got it! -- Yeah!!

# 7. Book Answer

Translation

```haskell
-- (𝜆𝑥𝑦𝑧.𝑥𝑧(𝑦𝑧))(𝜆𝑥.𝑧)(𝜆𝑥.𝑎)
(λxyz.xz(yz))(λx.z)(λx.a)

-- (𝜆𝑥.𝜆𝑦.𝜆𝑧.𝑥𝑧(𝑦𝑧))(𝜆𝑥.𝑧)(𝜆𝑥.𝑎)
(λx.λy.λz.xz(yz))(λx.z)(λx.a)

-- (𝜆𝑦.𝜆𝑧1.(𝜆𝑥.𝑧)𝑧1(𝑦𝑧1))(𝜆𝑥.𝑎)
(λy.λz1.(λx.z)z1(yz1))(λx.a)

-- (𝜆𝑧1.(𝜆𝑥.𝑧)(𝑧1)((𝜆𝑥.𝑎)𝑧1))
(λz1.(λx.z)(z1)((λx.a)z1))

-- (𝜆𝑧1.𝑧((𝜆𝑥.𝑎)(𝑧1)))
(λz1.z((λx.a)(z1)))

-- (𝜆𝑧1.𝑧𝑎)
(λz1.za)
```

Just answer

```haskell
(λxyz.xz(yz))(λx.z)(λx.a)

(λx.λy.λz.xz(yz))(λx.z)(λx.a)

(λy.λz1.(λx.z)z1(yz1))(λx.a)
--  apply λy to (λx.a)
(λz1.(λx.z)(z1)((λx.a)z1))
-- apply λx to fist (z1)
(λz1.z((λx.a)(z1)))
-- apply λx to (z1)
(λz1.za)
```

Analyze 1

```haskell
(λxyz.xz(yz))(λx.z)(λx.a)



(λx.λy.λz.xz(yz)) (λx.z) (λx.a)

(λy.λz1.(λx.z) z1 (yz1)) (λx.a)

(λz1.(λx.z) (z1) ((λx.a)z1))

(λz1.z ((λx.a) (z1)))

(λz1.za)
```
